Adapted TemplateToPCUIC (most is todo, corrected statement of translation theorem though)

pcuic/theories/TemplateToPCUIC.v
@@ -57,10 +57,12 @@ Section Trans.
                   idecl.(ind_ctors) brs' in
       tCase ci tp (trans c) tbrs
     | None => 
-      (** We build an ill-formed case if the term + environment are not well-formed *)
+      (** We build an ill-formed case if the term + environment are not well-formed.
+          But we still give the right length to the context so that all syntactic operations
+          still work. *)
       tCase ci {| pparams := p'.(Ast.pparams);
                   puinst := p'.(Ast.puinst);
-                  pcontext := [];
+                  pcontext := map (fun na => vass na (tSort Universe.type0)) p'.(Ast.pcontext);
                   preturn := p'.(Ast.preturn) |}
           (trans c) []
     end
@@ -75,52 +77,52 @@ Section Trans.
   | Ast.tFloat n => tPrim (primFloat; primFloatModel (float64_to_model n))
   end.
 
-  Definition trans_decl (d : Ast.context_decl) :=
+  Definition trans_decl (d : Ast.Env.context_decl) :=
     let 'mkdecl na b t := d in
     {| decl_name := na;
       decl_body := option_map trans b;
       decl_type := trans t |}.
 
   Definition trans_local Γ := List.map trans_decl Γ.
+  
+  Definition trans_constructor_body (d : Ast.Env.constructor_body) :=
+    {| cstr_name := d.(Ast.Env.cstr_name); 
+      cstr_args := trans_local d.(Ast.Env.cstr_args);
+      cstr_indices := map trans d.(Ast.Env.cstr_indices); 
+      cstr_type := trans d.(Ast.Env.cstr_type);
+      cstr_arity := d.(Ast.Env.cstr_arity) |}.
 
-  Definition trans_constructor_body (d : Ast.constructor_body) :=
-    {| cstr_name := d.(Ast.cstr_name); 
-      cstr_args := trans_local d.(Ast.cstr_args);
-      cstr_indices := map trans d.(Ast.cstr_indices); 
-      cstr_type := trans d.(Ast.cstr_type);
-      cstr_arity := d.(Ast.cstr_arity) |}.
-
-  Definition trans_one_ind_body (d : Ast.one_inductive_body) :=
-    {| ind_name := d.(Ast.ind_name);
-      ind_relevance := d.(Ast.ind_relevance);
-      ind_indices := trans_local d.(Ast.ind_indices);
-      ind_sort := d.(Ast.ind_sort);
-      ind_type := trans d.(Ast.ind_type);
-      ind_kelim := d.(Ast.ind_kelim);
-      ind_ctors := List.map trans_constructor_body d.(Ast.ind_ctors);
-      ind_projs := List.map (fun '(x, y) => (x, trans y)) d.(Ast.ind_projs) |}.
+  Definition trans_one_ind_body (d : Ast.Env.one_inductive_body) :=
+    {| ind_name := d.(Ast.Env.ind_name);
+      ind_relevance := d.(Ast.Env.ind_relevance);
+      ind_indices := trans_local d.(Ast.Env.ind_indices);
+      ind_sort := d.(Ast.Env.ind_sort);
+      ind_type := trans d.(Ast.Env.ind_type);
+      ind_kelim := d.(Ast.Env.ind_kelim);
+      ind_ctors := List.map trans_constructor_body d.(Ast.Env.ind_ctors);
+      ind_projs := List.map (fun '(x, y) => (x, trans y)) d.(Ast.Env.ind_projs) |}.
 
   Definition trans_constant_body bd :=
-    {| cst_type := trans bd.(Ast.cst_type); cst_body := option_map trans bd.(Ast.cst_body);
-      cst_universes := bd.(Ast.cst_universes) |}.
+    {| cst_type := trans bd.(Ast.Env.cst_type); cst_body := option_map trans bd.(Ast.Env.cst_body);
+      cst_universes := bd.(Ast.Env.cst_universes) |}.
 
   Definition trans_minductive_body md :=
-    {| ind_finite := md.(Ast.ind_finite);
-      ind_npars := md.(Ast.ind_npars);
-      ind_params := trans_local md.(Ast.ind_params);
-      ind_bodies := map trans_one_ind_body md.(Ast.ind_bodies);
-      ind_universes := md.(Ast.ind_universes);
-      ind_variance := md.(Ast.ind_variance) |}.
+    {| ind_finite := md.(Ast.Env.ind_finite);
+      ind_npars := md.(Ast.Env.ind_npars);
+      ind_params := trans_local md.(Ast.Env.ind_params);
+      ind_bodies := map trans_one_ind_body md.(Ast.Env.ind_bodies);
+      ind_universes := md.(Ast.Env.ind_universes);
+      ind_variance := md.(Ast.Env.ind_variance) |}.
 
-  Definition trans_global_decl (d : Ast.global_decl) :=
+  Definition trans_global_decl (d : Ast.Env.global_decl) :=
     match d with
-    | Ast.ConstantDecl bd => ConstantDecl (trans_constant_body bd)
-    | Ast.InductiveDecl bd => InductiveDecl (trans_minductive_body bd)
+    | Ast.Env.ConstantDecl bd => ConstantDecl (trans_constant_body bd)
+    | Ast.Env.InductiveDecl bd => InductiveDecl (trans_minductive_body bd)
     end.
 End Trans.
 
-Definition trans_global_decls (d : Ast.global_env) :=
+Definition trans_global_decls (d : Ast.Env.global_env) : global_env :=
   fold_right (fun decl Σ' => on_snd (trans_global_decl Σ') decl :: Σ') [] d.
 
-Definition trans_global (Σ : Ast.global_env_ext) :=
+Definition trans_global (Σ : Ast.Env.global_env_ext) : global_env_ext :=
   (trans_global_decls (fst Σ), snd Σ).
